$\max$ | $\displaystyle\lambda\sum_{i=1}^n \mu_i x_i - \frac{1}{S}\sum_{s=1}^S \left|\sum_{i=1}^n (R_i^s - \mu_i) x_i\right|$ |

$\mbox{subject to}$ | $\displaystyle\sum_{i=1}^n x_i = 1$ |

$x_1, \ldots, x_n\geq 0$ |

$\max$ | $\displaystyle\lambda\sum_{i=1}^n \mu_i x_i - \frac{1}{S}\sum_{s=1}^S \left(u_s^+ + u_s^-\right)$ |

$\mbox{subject to}$ | $\displaystyle\sum_{i=1}^n x_i = 1$ |

$u_s^+ - u_s^- = \displaystyle \sum_{i=1}^n (R_i^s - \mu_i) x_i$ for $s=1, \ldots, S$ | |

$x_1, \ldots, x_n, u_s^+, u_s^-\geq 0$ for $s=1, \ldots, S$. |